@prefix rdf: <http://www.w3.org/1999/02/22-rdf-syntax-ns#> .
@prefix rdfs: <http://www.w3.org/2000/01/rdf-schema#> .
@prefix skos: <http://www.w3.org/2004/02/skos/core#> .
@prefix skosxl: <http://www.w3.org/2008/05/skos-xl#> .
@prefix owl: <http://www.w3.org/2002/07/owl#> .
@prefix dc: <http://purl.org/dc/elements/1.1/> .
@prefix dcterms: <http://purl.org/dc/terms/> .
@prefix xsd: <http://www.w3.org/2001/XMLSchema#> .
@prefix tags: <http://www.holygoat.co.uk/owl/redwood/0.1/tags/> .
@prefix foaf: <http://xmlns.com/foaf/0.1/> .
@prefix cycAnnot: <http://sw.cyc.com/CycAnnotations_v1#> .
@prefix csw: <http://semantic-web.at/ontologies/csw.owl#> .
@prefix dbpedia: <http://dbpedia.org/resource/> .
@prefix freebase: <http://rdf.freebase.com/ns/> .
@prefix opencyc: <http://sw.opencyc.org/concept/> .
@prefix cyc: <http://sw.cyc.com/concept/> .
@prefix ctag: <http://commontag.org/ns#> .

<http://resource.geolba.ac.at/geoconnect3d/thesaurus> {<http://resource.geolba.ac.at/geoconnect3d/54> skos:notation "L1_08";
skos:definition "Join lines between ancient continents brought into juxtaposition by the consumption of an intervening ocean (Kearey and Vine, 1995)."@en;
skos:example "Iapetus suture"@en .
<http://resource.geolba.ac.at/geoconnect3d/55> a skos:Concept;
skos:prefLabel "Contact"@en .
<http://resource.geolba.ac.at/geoconnect3d/47> skos:narrower <http://resource.geolba.ac.at/geoconnect3d/55> .
<http://resource.geolba.ac.at/geoconnect3d/55> skos:broader <http://resource.geolba.ac.at/geoconnect3d/47>;
dcterms:created "2020-02-18T12:14:40.051Z"^^xsd:dateTime;
skos:notation "L1_09";
skos:definition "A plane or irregular surface other than a fault."@en .
<http://resource.geolba.ac.at/geoconnect3d/56> a skos:Concept;
skos:prefLabel "Limit level 2"@en .
<http://resource.geolba.ac.at/geoconnect3d/27> skos:hasTopConcept <http://resource.geolba.ac.at/geoconnect3d/56> .
<http://resource.geolba.ac.at/geoconnect3d/56> skos:topConceptOf <http://resource.geolba.ac.at/geoconnect3d/27>;
dcterms:created "2020-02-18T12:14:40.105Z"^^xsd:dateTime;
skos:notation "L2_01";
skos:definition "Detailing of the different types of \"Limit level 1\"."@en;
skos:scopeNote "Limits can be boundaries to units"@en .
<http://resource.geolba.ac.at/geoconnect3d/57> a skos:Concept;
skos:prefLabel "Shear zone"@en .
<http://resource.geolba.ac.at/geoconnect3d/56> skos:narrower <http://resource.geolba.ac.at/geoconnect3d/57> .
<http://resource.geolba.ac.at/geoconnect3d/57> skos:broader <http://resource.geolba.ac.at/geoconnect3d/56>;
dcterms:created "2020-02-18T12:14:40.177Z"^^xsd:dateTime;
skos:notation "L2_02";
skos:definition "Broad planar zone of relatively intense localised deformation (shearing) in which progressive deformation is non-coaxial (Passchier and Trouw, 1996; Hintersberger et al., 2017), and in which deformation is dominated by ductile deformation mechanisms (Schultz and Fossen, 2008)."@en .
<http://resource.geolba.ac.at/geoconnect3d/58> a skos:Concept;
skos:prefLabel "Normal fault"@en .
<http://resource.geolba.ac.at/geoconnect3d/56> skos:narrower <http://resource.geolba.ac.at/geoconnect3d/58> .
<http://resource.geolba.ac.at/geoconnect3d/58> skos:broader <http://resource.geolba.ac.at/geoconnect3d/56>;
dcterms:created "2020-02-18T12:14:40.271Z"^^xsd:dateTime;
skos:notation "L2_03";
skos:definition "concepts to be tuned with HIKE"@en .
<http://resource.geolba.ac.at/geoconnect3d/59> a skos:Concept;
skos:prefLabel "Reverse fault"@en .
<http://resource.geolba.ac.at/geoconnect3d/56> skos:narrower <http://resource.geolba.ac.at/geoconnect3d/59> .
<http://resource.geolba.ac.at/geoconnect3d/59> skos:broader <http://resource.geolba.ac.at/geoconnect3d/56>;
dcterms:created "2020-02-18T12:14:40.332Z"^^xsd:dateTime;
skos:notation "L2_04";
skos:definition "concepts to be tuned with HIKE"@en .
<http://resource.geolba.ac.at/geoconnect3d/60> a skos:Concept;
skos:prefLabel "Strike slip fault"@en .
<http://resource.geolba.ac.at/geoconnect3d/56> skos:narrower <http://resource.geolba.ac.at/geoconnect3d/60> .
<http://resource.geolba.ac.at/geoconnect3d/60> skos:broader <http://resource.geolba.ac.at/geoconnect3d/56>;
dcterms:created "2020-02-18T12:14:40.391Z"^^xsd:dateTime;
skos:notation "L2_05";
skos:definition "concepts to be tuned with HIKE"@en .
<http://resource.geolba.ac.at/geoconnect3d/61> a skos:Concept;
skos:prefLabel "Thrust fault"@en .
<http://resource.geolba.ac.at/geoconnect3d/56> skos:narrower <http://resource.geolba.ac.at/geoconnect3d/61> .
<http://resource.geolba.ac.at/geoconnect3d/61> skos:broader <http://resource.geolba.ac.at/geoconnect3d/56>;
dcterms:created "2020-02-18T12:14:40.443Z"^^xsd:dateTime;
skos:notation "L2_06";
skos:definition "concepts to be tuned with HIKE"@en .
<http://resource.geolba.ac.at/geoconnect3d/62> a skos:Concept;
skos:prefLabel "Detachment fault"@en .
<http://resource.geolba.ac.at/geoconnect3d/56> skos:narrower <http://resource.geolba.ac.at/geoconnect3d/62> .
<http://resource.geolba.ac.at/geoconnect3d/62> skos:broader <http://resource.geolba.ac.at/geoconnect3d/56>;
dcterms:created "2020-02-18T12:14:40.502Z"^^xsd:dateTime;
skos:notation "L2_07";
skos:definition "concepts to be tuned with HIKE"@en .
<http://resource.geolba.ac.at/geoconnect3d/63> a skos:Concept;
skos:prefLabel "Horizontal fault"@en .
<http://resource.geolba.ac.at/geoconnect3d/56> skos:narrower <http://resource.geolba.ac.at/geoconnect3d/63> .
<http://resource.geolba.ac.at/geoconnect3d/63> skos:broader <http://resource.geolba.ac.at/geoconnect3d/56>;
dcterms:created "2020-02-18T12:14:40.552Z"^^xsd:dateTime;
skos:notation "L2_08";
skos:definition "concepts to be tuned with HIKE"@en .
<http://resource.geolba.ac.at/geoconnect3d/64> a skos:Concept;
skos:prefLabel "Extraction fault"@en .
<http://resource.geolba.ac.at/geoconnect3d/56> skos:narrower <http://resource.geolba.ac.at/geoconnect3d/64> .
<http://resource.geolba.ac.at/geoconnect3d/64> skos:broader <http://resource.geolba.ac.at/geoconnect3d/56>;
dcterms:created "2020-02-18T12:14:40.612Z"^^xsd:dateTime;
skos:notation "L2_09";
skos:definition "concepts to be tuned with HIKE"@en .
<http://resource.geolba.ac.at/geoconnect3d/65> a skos:Concept;
skos:prefLabel "Pure extraction fault"@en .
<http://resource.geolba.ac.at/geoconnect3d/56> skos:narrower <http://resource.geolba.ac.at/geoconnect3d/65> .
<http://resource.geolba.ac.at/geoconnect3d/65> skos:broader <http://resource.geolba.ac.at/geoconnect3d/56>;
dcterms:created "2020-02-18T12:14:40.702Z"^^xsd:dateTime;
skos:notation "L2_10";
skos:definition "concepts to be tuned with HIKE"@en .
<http://resource.geolba.ac.at/geoconnect3d/66> a skos:Concept;
skos:prefLabel "Mixed extraction fault"@en .
<http://resource.geolba.ac.at/geoconnect3d/56> skos:narrower <http://resource.geolba.ac.at/geoconnect3d/66> .
<http://resource.geolba.ac.at/geoconnect3d/66> skos:broader <http://resource.geolba.ac.at/geoconnect3d/56>;
dcterms:created "2020-02-18T12:14:40.821Z"^^xsd:dateTime;
skos:notation "L2_11";
skos:definition "concepts to be tuned with HIKE"@en .
<http://resource.geolba.ac.at/geoconnect3d/67> a skos:Concept;
skos:prefLabel "Oblique slip fault"@en .
<http://resource.geolba.ac.at/geoconnect3d/56> skos:narrower <http://resource.geolba.ac.at/geoconnect3d/67> .
<http://resource.geolba.ac.at/geoconnect3d/67> skos:broader <http://resource.geolba.ac.at/geoconnect3d/56>;
dcterms:created "2020-02-18T12:14:40.862Z"^^xsd:dateTime;
skos:notation "L2_12";
skos:definition "concepts to be tuned with HIKE"@en .
<http://resource.geolba.ac.at/geoconnect3d/68> a skos:Concept;
skos:prefLabel "Scissor fault"@en .
<http://resource.geolba.ac.at/geoconnect3d/56> skos:narrower <http://resource.geolba.ac.at/geoconnect3d/68> .
<http://resource.geolba.ac.at/geoconnect3d/68> skos:broader <http://resource.geolba.ac.at/geoconnect3d/56>;
dcterms:created "2020-02-18T12:14:40.895Z"^^xsd:dateTime;
skos:notation "L2_13";
skos:definition "concepts to be tuned with HIKE"@en .
<http://resource.geolba.ac.at/geoconnect3d/69> a skos:Concept;
skos:prefLabel "Wrench fault"@en .
<http://resource.geolba.ac.at/geoconnect3d/56> skos:narrower <http://resource.geolba.ac.at/geoconnect3d/69> .
<http://resource.geolba.ac.at/geoconnect3d/69> skos:broader <http://resource.geolba.ac.at/geoconnect3d/56>;
dcterms:created "2020-02-18T12:14:40.955Z"^^xsd:dateTime;
skos:notation "L2_14";
skos:definition "concepts to be tuned with HIKE"@en;
skos:notation "L2_15";
skos:definition "Broad planar zone of relatively intense localised deformation (shearing) in which progressive deformation is non-coaxial (Passchier and Trouw, 1996; Hintersberger et al., 2017), and in which deformation is dominated by ductile deformation mechanisms (Schultz and Fossen, 2008)."@en .
<http://resource.geolba.ac.at/geoconnect3d/70> a skos:Concept;
skos:prefLabel "Active plate boundary"@en .
<http://resource.geolba.ac.at/geoconnect3d/56> skos:narrower <http://resource.geolba.ac.at/geoconnect3d/70> .
<http://resource.geolba.ac.at/geoconnect3d/70> skos:broader <http://resource.geolba.ac.at/geoconnect3d/56>;
dcterms:created "2020-02-18T12:14:41.018Z"^^xsd:dateTime;
skos:notation "L2_16";
skos:definition "to be defined"@en .
<http://resource.geolba.ac.at/geoconnect3d/71> a skos:Concept;
skos:prefLabel "Passive plate boundary"@en .
<http://resource.geolba.ac.at/geoconnect3d/56> skos:narrower <http://resource.geolba.ac.at/geoconnect3d/71> .
<http://resource.geolba.ac.at/geoconnect3d/71> skos:broader <http://resource.geolba.ac.at/geoconnect3d/56>;
dcterms:created "2020-02-18T12:14:41.076Z"^^xsd:dateTime;
skos:notation "L2_17";
skos:definition "to be defined"@en .
<http://resource.geolba.ac.at/geoconnect3d/72> a skos:Concept;
skos:prefLabel "Suture"@en .
<http://resource.geolba.ac.at/geoconnect3d/56> skos:narrower <http://resource.geolba.ac.at/geoconnect3d/72> .
<http://resource.geolba.ac.at/geoconnect3d/72> skos:broader <http://resource.geolba.ac.at/geoconnect3d/56>;
dcterms:created "2020-02-18T12:14:41.119Z"^^xsd:dateTime;
skos:notation "L2_18";
skos:definition "Join lines between ancient continents brought into juxtaposition by the consumption of an intervening ocean (Kearey and Vine, 1995)."@en .
<http://resource.geolba.ac.at/geoconnect3d/73> a skos:Concept;
skos:prefLabel "Unconformity"@en .
<http://resource.geolba.ac.at/geoconnect3d/56> skos:narrower <http://resource.geolba.ac.at/geoconnect3d/73> .
<http://resource.geolba.ac.at/geoconnect3d/73> skos:broader <http://resource.geolba.ac.at/geoconnect3d/56>;
dcterms:created "2020-02-18T12:14:41.189Z"^^xsd:dateTime;
skos:notation "L2_19";
skos:definition "Surface between rock units where one is overlain by another that is not next in the stratigraphic succession due to substantial break or gap in the geologic record (Neuendorf et al., 2005)."@en .
<http://resource.geolba.ac.at/geoconnect3d/74> a skos:Concept;
skos:prefLabel "Stratigraphic contact"@en .
<http://resource.geolba.ac.at/geoconnect3d/56> skos:narrower <http://resource.geolba.ac.at/geoconnect3d/74> .
<http://resource.geolba.ac.at/geoconnect3d/74> skos:broader <http://resource.geolba.ac.at/geoconnect3d/56>;
dcterms:created "2020-02-18T12:14:41.220Z"^^xsd:dateTime;
skos:notation "L2_20";
skos:definition "Plane or irregular surface between two types or ages of rock (adapted from Neuendorf et al., 2005)."@en .
<http://resource.geolba.ac.at/geoconnect3d/75> a skos:Concept;
skos:prefLabel "Magmatic contact"@en .
<http://resource.geolba.ac.at/geoconnect3d/56> skos:narrower <http://resource.geolba.ac.at/geoconnect3d/75> .
<http://resource.geolba.ac.at/geoconnect3d/75> skos:broader <http://resource.geolba.ac.at/geoconnect3d/56>;
dcterms:created "2020-02-18T12:14:41.257Z"^^xsd:dateTime;
skos:notation "L2_21";
skos:definition "Plane or irregular surface between a group of related magmatic rocks and their country rock(s)."@en .
<http://resource.geolba.ac.at/geoconnect3d/0> a skos:ConceptScheme;
dcterms:created "2020-02-07T14:36:28.944Z"^^xsd:dateTime .
<http://resource.geolba.ac.at/geoconnect3d/1> a skos:Concept;
skos:prefLabel "RVG large-scale fault system"@en .
<http://resource.geolba.ac.at/geoconnect3d/0> skos:hasTopConcept <http://resource.geolba.ac.at/geoconnect3d/1> .
<http://resource.geolba.ac.at/geoconnect3d/1> skos:topConceptOf <http://resource.geolba.ac.at/geoconnect3d/0>;
dcterms:created "2020-02-07T14:36:28.977Z"^^xsd:dateTime;
skos:definition "Faults part of the larger RVG with common activity during the Kimmerian, Subhercynic or Cenozoïc tectonic phases."@en .
<http://resource.geolba.ac.at/geoconnect3d/2> a skos:Concept;
skos:prefLabel "Feldbiss fault system"@en .
<http://resource.geolba.ac.at/geoconnect3d/1> skos:narrower <http://resource.geolba.ac.at/geoconnect3d/2> .
<http://resource.geolba.ac.at/geoconnect3d/2> skos:broader <http://resource.geolba.ac.at/geoconnect3d/1>;
dcterms:created "2020-02-07T14:36:29.010Z"^^xsd:dateTime;
skos:notation "VITO_001";
skos:definition "Group of normal faults defining the western border of the RVG with common activity during the Cenozoic extension and a minimal vertical throw of 100m."@en .
<http://resource.geolba.ac.at/geoconnect3d/3> a skos:Concept;
skos:prefLabel "Neeroeteren-Grote_Brogel_O-Overpelt"@en .
<http://resource.geolba.ac.at/geoconnect3d/2> skos:narrower <http://resource.geolba.ac.at/geoconnect3d/3> .
<http://resource.geolba.ac.at/geoconnect3d/3> skos:broader <http://resource.geolba.ac.at/geoconnect3d/2>;
dcterms:created "2020-02-07T14:36:29.037Z"^^xsd:dateTime;
skos:notation "VITO_002";
skos:definition "Normal fault in the RVG large-scale fault system active during the Kimmerian phase,  reactivated as a reverse fault during the Subhercynic inversion phase and finally reactivated  as a normal fault again during the Cenozoic extension."@en .
<http://resource.geolba.ac.at/geoconnect3d/4> a skos:Concept;
skos:prefLabel "Grote_Brogel_W"@en .
<http://resource.geolba.ac.at/geoconnect3d/2> skos:narrower <http://resource.geolba.ac.at/geoconnect3d/4> .
<http://resource.geolba.ac.at/geoconnect3d/4> skos:broader <http://resource.geolba.ac.at/geoconnect3d/2>;
dcterms:created "2020-02-07T14:36:29.065Z"^^xsd:dateTime;
skos:notation "VITO_003";
skos:definition "Normal fault in the RVG large-scale fault system active during the Kimmerian phase,  reactivated as a reverse fault during the Subhercynic inversion phase and finally reactivated  as a normal fault again during the Cenozoic extension."@en .
<http://resource.geolba.ac.at/geoconnect3d/5> a skos:Concept;
skos:prefLabel "Bocholt"@en .
<http://resource.geolba.ac.at/geoconnect3d/2> skos:narrower <http://resource.geolba.ac.at/geoconnect3d/5> .
<http://resource.geolba.ac.at/geoconnect3d/5> skos:broader <http://resource.geolba.ac.at/geoconnect3d/2>;
dcterms:created "2020-02-07T14:36:29.093Z"^^xsd:dateTime;
skos:notation "VITO_004";
skos:definition "Normal fault in the RVG large-scale fault system active during the Kimmerian phase and reactivated  as a normal fault during the Cenozoic extension."@en .
<http://resource.geolba.ac.at/geoconnect3d/6> a skos:Concept;
skos:prefLabel "Hamont"@en .
<http://resource.geolba.ac.at/geoconnect3d/2> skos:narrower <http://resource.geolba.ac.at/geoconnect3d/6> .
<http://resource.geolba.ac.at/geoconnect3d/6> skos:broader <http://resource.geolba.ac.at/geoconnect3d/2>;
dcterms:created "2020-02-07T14:36:29.121Z"^^xsd:dateTime;
skos:notation "VITO_005";
skos:definition "Normal fault in the RVG large-scale fault system active during the Kimmerian phase and reactivated  as a normal fault during the Cenozoic extension."@en .
<http://resource.geolba.ac.at/geoconnect3d/7> a skos:Concept;
skos:prefLabel "Reppel"@en .
<http://resource.geolba.ac.at/geoconnect3d/2> skos:narrower <http://resource.geolba.ac.at/geoconnect3d/7> .
<http://resource.geolba.ac.at/geoconnect3d/7> skos:broader <http://resource.geolba.ac.at/geoconnect3d/2>;
dcterms:created "2020-02-07T14:36:29.148Z"^^xsd:dateTime;
skos:notation "VITO_006";
skos:definition "Normal fault in the RVG large-scale fault system active during the Kimmerian phase and reactivated  as a normal fault during the Cenozoic extension."@en .
<http://resource.geolba.ac.at/geoconnect3d/8> a skos:Concept;
skos:prefLabel "Rotem"@en .
<http://resource.geolba.ac.at/geoconnect3d/2> skos:narrower <http://resource.geolba.ac.at/geoconnect3d/8> .
<http://resource.geolba.ac.at/geoconnect3d/8> skos:broader <http://resource.geolba.ac.at/geoconnect3d/2>;
dcterms:created "2020-02-07T14:36:29.176Z"^^xsd:dateTime;
skos:notation "VITO_007";
skos:definition "Normal fault in the RVG large-scale fault system active during the Kimmerian phase,  reactivated as a reverse fault during the Subhercynic inversion phase and finally reactivated  as a normal fault again during the Cenozoic extension."@en .
<http://resource.geolba.ac.at/geoconnect3d/9> a skos:Concept;
skos:prefLabel "Cenozoic faults in the RVG large-scale fault system"@en .
<http://resource.geolba.ac.at/geoconnect3d/1> skos:narrower <http://resource.geolba.ac.at/geoconnect3d/9> .
<http://resource.geolba.ac.at/geoconnect3d/9> skos:broader <http://resource.geolba.ac.at/geoconnect3d/1>;
dcterms:created "2020-02-07T14:36:29.204Z"^^xsd:dateTime;
skos:notation "VITO_008";
skos:definition "Group of faults situated within the RVG large-scale fault system for which the known activity is limited to the Cenozoic extension."@en .
<http://resource.geolba.ac.at/geoconnect3d/10> a skos:Concept;
skos:prefLabel "Reactivated Mesozoic faults in the RVG large-scale fault system"@en .
<http://resource.geolba.ac.at/geoconnect3d/1> skos:narrower <http://resource.geolba.ac.at/geoconnect3d/10> .
<http://resource.geolba.ac.at/geoconnect3d/10> skos:broader <http://resource.geolba.ac.at/geoconnect3d/1>;
dcterms:created "2020-02-07T14:36:29.232Z"^^xsd:dateTime;
skos:notation "VITO_009";
skos:definition "Group of faults situated within the RVG large-scale fault system with known activity during the Kimmerian phase and the Cenozoic extension."@en .
<http://resource.geolba.ac.at/geoconnect3d/11> a skos:Concept;
skos:prefLabel "Non-reactivated Subhercynic faults in the RVG large-scale faultsystem"@en .
<http://resource.geolba.ac.at/geoconnect3d/1> skos:narrower <http://resource.geolba.ac.at/geoconnect3d/11> .
<http://resource.geolba.ac.at/geoconnect3d/11> skos:broader <http://resource.geolba.ac.at/geoconnect3d/1>;
dcterms:created "2020-02-07T14:36:29.262Z"^^xsd:dateTime;
skos:notation "VITO_010";
skos:definition "Group of reverse- and thrust faults faults situated within the RVG large-scale fault system with activity limited to the Subhercynic inversion phase."@en .
<http://resource.geolba.ac.at/geoconnect3d/12> a skos:Concept;
skos:prefLabel "Campine block"@en .
<http://resource.geolba.ac.at/geoconnect3d/0> skos:hasTopConcept <http://resource.geolba.ac.at/geoconnect3d/12> .
<http://resource.geolba.ac.at/geoconnect3d/12> skos:topConceptOf <http://resource.geolba.ac.at/geoconnect3d/0>;
dcterms:created "2020-02-07T14:36:29.290Z"^^xsd:dateTime;
skos:notation "VITO_021";
skos:definition "Faults part of the Campine block with common activity during the Kimmerian and/or Cenozoic tectonic phases."@en .
<http://resource.geolba.ac.at/geoconnect3d/13> a skos:Concept;
skos:prefLabel "Cenozoic faults in the Campine block"@en .
<http://resource.geolba.ac.at/geoconnect3d/12> skos:narrower <http://resource.geolba.ac.at/geoconnect3d/13> .
<http://resource.geolba.ac.at/geoconnect3d/13> skos:broader <http://resource.geolba.ac.at/geoconnect3d/12>;
dcterms:created "2020-02-07T14:36:29.318Z"^^xsd:dateTime;
skos:notation "VITO_011";
skos:definition "Group of faults situated within the Campine block for which the known activity is limited to the Cenozoic."@en .
<http://resource.geolba.ac.at/geoconnect3d/14> a skos:Concept;
skos:prefLabel "Faults in the Campine block  with a Mesozoic throw of less than 200m and a Cenozoic throw"@en .
<http://resource.geolba.ac.at/geoconnect3d/12> skos:narrower <http://resource.geolba.ac.at/geoconnect3d/14> .
<http://resource.geolba.ac.at/geoconnect3d/14> skos:broader <http://resource.geolba.ac.at/geoconnect3d/12>;
dcterms:created "2020-02-07T14:36:29.347Z"^^xsd:dateTime;
skos:notation "VITO_012";
skos:definition "Group of faults situated within the Campine block with known activity during the Kimmerian phase and Cenozoic extension. The faults all have a Cenozoic throw and their Mesozoic throw is less than 200 m."@en .
<http://resource.geolba.ac.at/geoconnect3d/15> a skos:Concept;
skos:prefLabel "Faults in the Campine block  with a Mesozoic throw of more than 200m and a Cenozoic throw"@en .
<http://resource.geolba.ac.at/geoconnect3d/12> skos:narrower <http://resource.geolba.ac.at/geoconnect3d/15> .
<http://resource.geolba.ac.at/geoconnect3d/15> skos:broader <http://resource.geolba.ac.at/geoconnect3d/12>;
dcterms:created "2020-02-07T14:36:29.376Z"^^xsd:dateTime;
skos:notation "VITO_013";
skos:definition "Group of faults situated within the Campine block with known activity during the Kimmerian phase and Cenozoic extension.The faults all have a Cenozoic throw and their  Mesozoic throw is more than 200 m."@en .
<http://resource.geolba.ac.at/geoconnect3d/16> a skos:Concept;
skos:prefLabel "Faults in the Campine block  with a Mesozoic throw of less than 200m and no Cenozoic throw"@en .
<http://resource.geolba.ac.at/geoconnect3d/12> skos:narrower <http://resource.geolba.ac.at/geoconnect3d/16> .
<http://resource.geolba.ac.at/geoconnect3d/16> skos:broader <http://resource.geolba.ac.at/geoconnect3d/12>;
dcterms:created "2020-02-07T14:36:29.405Z"^^xsd:dateTime;
skos:notation "VITO_014";
skos:definition "Group of faults situated within the Campine block with known activity during the Kimmerian phase and Cenozoic extension. The faults have no throw in the Cenozoic  and their Mesozoic throw is less than 200m. The throw related to the Cenozoic extension can be local and is limited to the Upper Cretaceous."@en .
<http://resource.geolba.ac.at/geoconnect3d/17> a skos:Concept;
skos:prefLabel "Faults in the Campine block  with a Mesozoic throw of more than 200m and no Cenozoic throw"@en .
<http://resource.geolba.ac.at/geoconnect3d/12> skos:narrower <http://resource.geolba.ac.at/geoconnect3d/17> .
<http://resource.geolba.ac.at/geoconnect3d/17> skos:broader <http://resource.geolba.ac.at/geoconnect3d/12>;
dcterms:created "2020-02-07T14:36:29.433Z"^^xsd:dateTime;
skos:notation "VITO_015";
skos:definition "Group of faults situated within the Campine block with known activity during the Kimmerian phase and Cenozoic extension. The faults have no throw in the Cenozoic  and their Mesozoic throw is more than 200m. The throw related to the Cenozoic extension can be local and is limited to the Upper Cretaceous."@en .
<http://resource.geolba.ac.at/geoconnect3d/18> a skos:Concept;
skos:prefLabel "Non-reactivated Mesozoic faults in the Campine block with a throw of less than 200m"@en .
<http://resource.geolba.ac.at/geoconnect3d/12> skos:narrower <http://resource.geolba.ac.at/geoconnect3d/18> .
<http://resource.geolba.ac.at/geoconnect3d/18> skos:broader <http://resource.geolba.ac.at/geoconnect3d/12>;
dcterms:created "2020-02-07T14:36:29.461Z"^^xsd:dateTime;
skos:notation "VITO_016";
skos:definition "Group of faults situated within the Campine block with activity limited to the Kimmerian phase."@en .
<http://resource.geolba.ac.at/geoconnect3d/19> a skos:Concept;
skos:prefLabel "Non-reactivated Mesozoic faults in the Campine block with a throw of more than 200m"@en .
<http://resource.geolba.ac.at/geoconnect3d/12> skos:narrower <http://resource.geolba.ac.at/geoconnect3d/19> .
<http://resource.geolba.ac.at/geoconnect3d/19> skos:broader <http://resource.geolba.ac.at/geoconnect3d/12>;
dcterms:created "2020-02-07T14:36:29.489Z"^^xsd:dateTime;
skos:notation "VITO_017";
skos:definition "Group of faults situated within the Campine block with activity limited to the Kimmerian phase and  a throw of more than 200m."@en .
<http://resource.geolba.ac.at/geoconnect3d/20> a skos:Concept;
skos:prefLabel "Hoogstraten fault"@en .
<http://resource.geolba.ac.at/geoconnect3d/12> skos:narrower <http://resource.geolba.ac.at/geoconnect3d/20> .
<http://resource.geolba.ac.at/geoconnect3d/20> skos:broader <http://resource.geolba.ac.at/geoconnect3d/12>;
dcterms:created "2020-02-07T14:36:29.517Z"^^xsd:dateTime;
skos:notation "VITO_018";
skos:definition "Major normal, listric fault within the Campine block, probably active during the Kimmerian phase with a distinct strike."@en .
<http://resource.geolba.ac.at/geoconnect3d/21> a skos:Concept;
skos:prefLabel "Rauw fault"@en .
<http://resource.geolba.ac.at/geoconnect3d/12> skos:narrower <http://resource.geolba.ac.at/geoconnect3d/21> .
<http://resource.geolba.ac.at/geoconnect3d/21> skos:broader <http://resource.geolba.ac.at/geoconnect3d/12>;
dcterms:created "2020-02-07T14:36:29.545Z"^^xsd:dateTime;
skos:notation "VITO_019";
skos:definition "Major normal fault within the Campine block, active during the Kimmerian phase and the Cenozoïc extension. Influenced Pleistocene fluvial patterns, leading to Holocene relief inversion."@en .
<http://resource.geolba.ac.at/geoconnect3d/22> a skos:Concept;
skos:prefLabel "Rauw_2"@en .
<http://resource.geolba.ac.at/geoconnect3d/12> skos:narrower <http://resource.geolba.ac.at/geoconnect3d/22> .
<http://resource.geolba.ac.at/geoconnect3d/22> skos:broader <http://resource.geolba.ac.at/geoconnect3d/12>;
dcterms:created "2020-02-07T14:36:29.573Z"^^xsd:dateTime;
skos:notation "VITO_020";
skos:definition "Subfault of the Rauw fault."@en .
<http://resource.geolba.ac.at/geoconnect3d/23> a skos:ConceptScheme;
dcterms:created "2020-02-07T14:39:35.903Z"^^xsd:dateTime .
<http://resource.geolba.ac.at/geoconnect3d/47> skos:notation "L1_01";
skos:definition "A planar structure that limits a unit."@en;
skos:scopeNote "Limits can be boundaries to units"@en .
<http://resource.geolba.ac.at/geoconnect3d/48> a skos:Concept;
skos:prefLabel "Large-scale fault system"@en .
<http://resource.geolba.ac.at/geoconnect3d/25> a skos:Concept .
<http://resource.geolba.ac.at/geoconnect3d/47> skos:narrower <http://resource.geolba.ac.at/geoconnect3d/48> .
<http://resource.geolba.ac.at/geoconnect3d/25> dcterms:created "2020-02-07T14:40:38.202Z"^^xsd:dateTime;
skos:prefLabel "Dusar et al (2001)"@en .
<http://resource.geolba.ac.at/geoconnect3d/26> dcterms:created "2020-02-07T14:41:07.861Z"^^xsd:dateTime;
skos:prefLabel "Deckers et al (2019)"@en;
a skos:Concept .
<http://resource.geolba.ac.at/geoconnect3d/25> a dcterms:BibliographicResource .
<http://resource.geolba.ac.at/geoconnect3d/26> a dcterms:BibliographicResource .
<http://resource.geolba.ac.at/geoconnect3d/25> dcterms:bibliographicCitation "Dusar, M., Rijpens, J., Sintubin, M., & Wouters, L. (2001): Plio-Pleistocene fault pattern of the Feldbiss fault system (southern border of the Roer Valley Graben, Belgium) based on high resolution reflection seismic data. Geologie en Mijnbouw, 80(3/4), 79-94." .
<http://resource.geolba.ac.at/geoconnect3d/26> dcterms:bibliographicCitation "Deckers J., De Koninck R., Bos S., Broothaers M., Dirix K., Hambsch L., Lagrou, D., Lanckacker T., Matthijs, J., Rombaut B., Van Baelen K. & Van Haren T., (2019): Geologisch (G3D) en hydrogeologisch (H3D) 3D lagenmodel van Vlaanderen – versie 3. Studie uitgevoerd in opdracht van het Vlaams Planbureau voor Omgeving, departement Omgeving en de Vlaamse Milieumaatschappij. VITO-rapport 2018/RMA/R/1569. In review" .
<http://resource.geolba.ac.at/geoconnect3d/13> dcterms:references <http://resource.geolba.ac.at/geoconnect3d/26> .
<http://resource.geolba.ac.at/geoconnect3d/12> dcterms:references <http://resource.geolba.ac.at/geoconnect3d/26> .
<http://resource.geolba.ac.at/geoconnect3d/14> dcterms:references <http://resource.geolba.ac.at/geoconnect3d/26> .
<http://resource.geolba.ac.at/geoconnect3d/16> dcterms:references <http://resource.geolba.ac.at/geoconnect3d/26> .
<http://resource.geolba.ac.at/geoconnect3d/15> dcterms:references <http://resource.geolba.ac.at/geoconnect3d/26> .
<http://resource.geolba.ac.at/geoconnect3d/17> dcterms:references <http://resource.geolba.ac.at/geoconnect3d/26> .
<http://resource.geolba.ac.at/geoconnect3d/20> dcterms:references <http://resource.geolba.ac.at/geoconnect3d/26> .
<http://resource.geolba.ac.at/geoconnect3d/18> dcterms:references <http://resource.geolba.ac.at/geoconnect3d/26> .
<http://resource.geolba.ac.at/geoconnect3d/19> dcterms:references <http://resource.geolba.ac.at/geoconnect3d/26> .
<http://resource.geolba.ac.at/geoconnect3d/22> dcterms:references <http://resource.geolba.ac.at/geoconnect3d/26> .
<http://resource.geolba.ac.at/geoconnect3d/21> dcterms:references <http://resource.geolba.ac.at/geoconnect3d/26> .
<http://resource.geolba.ac.at/geoconnect3d/1> dcterms:references <http://resource.geolba.ac.at/geoconnect3d/26> .
<http://resource.geolba.ac.at/geoconnect3d/9> dcterms:references <http://resource.geolba.ac.at/geoconnect3d/26> .
<http://resource.geolba.ac.at/geoconnect3d/2> dcterms:references <http://resource.geolba.ac.at/geoconnect3d/26>,<http://resource.geolba.ac.at/geoconnect3d/25> .
<http://resource.geolba.ac.at/geoconnect3d/5> dcterms:references <http://resource.geolba.ac.at/geoconnect3d/25> .
<http://resource.geolba.ac.at/geoconnect3d/4> dcterms:references <http://resource.geolba.ac.at/geoconnect3d/25> .
<http://resource.geolba.ac.at/geoconnect3d/6> dcterms:references <http://resource.geolba.ac.at/geoconnect3d/25> .
<http://resource.geolba.ac.at/geoconnect3d/3> dcterms:references <http://resource.geolba.ac.at/geoconnect3d/25> .
<http://resource.geolba.ac.at/geoconnect3d/7> dcterms:references <http://resource.geolba.ac.at/geoconnect3d/25> .
<http://resource.geolba.ac.at/geoconnect3d/8> dcterms:references <http://resource.geolba.ac.at/geoconnect3d/25> .
<http://resource.geolba.ac.at/geoconnect3d/11> dcterms:references <http://resource.geolba.ac.at/geoconnect3d/26> .
<http://resource.geolba.ac.at/geoconnect3d/10> dcterms:references <http://resource.geolba.ac.at/geoconnect3d/26> .
<http://resource.geolba.ac.at/geoconnect3d/27> a skos:ConceptScheme;
dcterms:created "2020-02-18T12:14:38.188Z"^^xsd:dateTime .
<http://resource.geolba.ac.at/geoconnect3d/28> a skos:Concept;
skos:prefLabel "Unit level 1"@en .
<http://resource.geolba.ac.at/geoconnect3d/27> skos:hasTopConcept <http://resource.geolba.ac.at/geoconnect3d/28> .
<http://resource.geolba.ac.at/geoconnect3d/28> skos:topConceptOf <http://resource.geolba.ac.at/geoconnect3d/27>;
dcterms:created "2020-02-18T12:14:38.220Z"^^xsd:dateTime;
skos:notation "U1_01";
skos:definition "Rock mass with common structural or deformation features, mutual relations, origin or historical evolution. Contained material may be igneous, sedimentary, or metamorphic (Neuendorf et al., 2005)."@en .
<http://resource.geolba.ac.at/geoconnect3d/29> a skos:Concept;
skos:prefLabel "Basin system"@en .
<http://resource.geolba.ac.at/geoconnect3d/28> skos:narrower <http://resource.geolba.ac.at/geoconnect3d/29> .
<http://resource.geolba.ac.at/geoconnect3d/29> skos:broader <http://resource.geolba.ac.at/geoconnect3d/28>;
dcterms:created "2020-02-18T12:14:38.251Z"^^xsd:dateTime;
skos:notation "U1_02";
skos:definition "Group of tectonically-derived lower areas in which sediments have accumulated (Neuendorf et al., 2005)."@en .
<http://resource.geolba.ac.at/geoconnect3d/30> a skos:Concept;
skos:prefLabel "Basin"@en .
<http://resource.geolba.ac.at/geoconnect3d/29> skos:narrower <http://resource.geolba.ac.at/geoconnect3d/30> .
<http://resource.geolba.ac.at/geoconnect3d/30> skos:broader <http://resource.geolba.ac.at/geoconnect3d/29>;
dcterms:created "2020-02-18T12:14:38.282Z"^^xsd:dateTime;
skos:notation "U1_03";
skos:definition "Lower area in which sediments have accumulated (adapted from Neuendorf et al., 2005)."@en .
<http://resource.geolba.ac.at/geoconnect3d/31> a skos:Concept;
skos:prefLabel "Subbasin"@en .
<http://resource.geolba.ac.at/geoconnect3d/30> skos:narrower <http://resource.geolba.ac.at/geoconnect3d/31> .
<http://resource.geolba.ac.at/geoconnect3d/31> skos:broader <http://resource.geolba.ac.at/geoconnect3d/30>;
dcterms:created "2020-02-18T12:14:38.320Z"^^xsd:dateTime;
skos:notation "U1_04";
skos:definition "Area within a sedimentary basin that is partially separated by topographic effect or structurally elements (e.g. topographic heights or faults) from the rest of the basin (GBA, 2019)"@en .
<http://resource.geolba.ac.at/geoconnect3d/32> a skos:Concept;
skos:prefLabel "Magmatic complex"@en .
<http://resource.geolba.ac.at/geoconnect3d/28> skos:narrower <http://resource.geolba.ac.at/geoconnect3d/32> .
<http://resource.geolba.ac.at/geoconnect3d/32> skos:broader <http://resource.geolba.ac.at/geoconnect3d/28>;
dcterms:created "2020-02-18T12:14:38.362Z"^^xsd:dateTime;
skos:notation "U1_05";
skos:definition "Group of spatially related and possibly contemporaneous magmatic rocks (adapted from Neuendorf et al. 2005)."@en .
<http://resource.geolba.ac.at/geoconnect3d/33> a skos:Concept;
skos:prefLabel "Magmatic body"@en .
<http://resource.geolba.ac.at/geoconnect3d/32> skos:narrower <http://resource.geolba.ac.at/geoconnect3d/33> .
<http://resource.geolba.ac.at/geoconnect3d/33> skos:broader <http://resource.geolba.ac.at/geoconnect3d/32>;
dcterms:created "2020-02-18T12:14:38.403Z"^^xsd:dateTime;
skos:notation "U1_06";
skos:definition "Individual rock body part of a magmatic complex."@en .
<http://resource.geolba.ac.at/geoconnect3d/34> a skos:Concept;
skos:prefLabel "Orogen"@en .
<http://resource.geolba.ac.at/geoconnect3d/28> skos:narrower <http://resource.geolba.ac.at/geoconnect3d/34> .
<http://resource.geolba.ac.at/geoconnect3d/34> skos:broader <http://resource.geolba.ac.at/geoconnect3d/28>;
dcterms:created "2020-02-18T12:14:38.442Z"^^xsd:dateTime;
skos:notation "U1_07";
skos:definition "Broad region that has been subjected to folding and other deformation during an orogenic cycle (Neuendorf et al. 2005). Located along an anciant (destructive-converging) plate boundary (GBA, 2019)."@en .
<http://resource.geolba.ac.at/geoconnect3d/35> a skos:Concept;
skos:prefLabel "Plate"@en .
<http://resource.geolba.ac.at/geoconnect3d/28> skos:narrower <http://resource.geolba.ac.at/geoconnect3d/35> .
<http://resource.geolba.ac.at/geoconnect3d/35> skos:broader <http://resource.geolba.ac.at/geoconnect3d/28>;
dcterms:created "2020-02-18T12:14:38.500Z"^^xsd:dateTime;
skos:notation "U1_08";
skos:definition "part of an interlocking network of segments of the lithosphere with relative divergent, convergent or tangential movement"@en .
<http://resource.geolba.ac.at/geoconnect3d/36> a skos:Concept;
skos:prefLabel "Unit level 2"@en .
<http://resource.geolba.ac.at/geoconnect3d/27> skos:hasTopConcept <http://resource.geolba.ac.at/geoconnect3d/36> .
<http://resource.geolba.ac.at/geoconnect3d/36> skos:topConceptOf <http://resource.geolba.ac.at/geoconnect3d/27>;
dcterms:created "2020-02-18T12:14:38.630Z"^^xsd:dateTime;
skos:notation "U2_01";
skos:definition "Detailing of the different types of \"Unit level 1\"."@en .
<http://resource.geolba.ac.at/geoconnect3d/37> a skos:Concept;
skos:prefLabel "Graben"@en .
<http://resource.geolba.ac.at/geoconnect3d/36> skos:narrower <http://resource.geolba.ac.at/geoconnect3d/37> .
<http://resource.geolba.ac.at/geoconnect3d/37> skos:broader <http://resource.geolba.ac.at/geoconnect3d/36>;
dcterms:created "2020-02-18T12:14:38.664Z"^^xsd:dateTime;
skos:notation "U2_02";
skos:definition "Elongate, relatively depressed crustal unit or block bounded by faults on its long sides (Neuendorf et al., 2005)."@en .
<http://resource.geolba.ac.at/geoconnect3d/38> a skos:Concept;
skos:prefLabel "Horst"@en .
<http://resource.geolba.ac.at/geoconnect3d/36> skos:narrower <http://resource.geolba.ac.at/geoconnect3d/38> .
<http://resource.geolba.ac.at/geoconnect3d/38> skos:broader <http://resource.geolba.ac.at/geoconnect3d/36>;
dcterms:created "2020-02-18T12:14:38.749Z"^^xsd:dateTime;
skos:notation "U2_03";
skos:definition "Elongate, relatively uplifted crustal unit bounded by faults on its long sides (Neuendorf et al., 2005)."@en .
<http://resource.geolba.ac.at/geoconnect3d/39> a skos:Concept;
skos:prefLabel "Though"@en .
<http://resource.geolba.ac.at/geoconnect3d/36> skos:narrower <http://resource.geolba.ac.at/geoconnect3d/39> .
<http://resource.geolba.ac.at/geoconnect3d/39> skos:broader <http://resource.geolba.ac.at/geoconnect3d/36>;
dcterms:created "2020-02-18T12:14:38.808Z"^^xsd:dateTime;
skos:notation "U2_04";
skos:definition "Elongate, distinctively narrow, relatively depressed crustal unit."@en .
<http://resource.geolba.ac.at/geoconnect3d/40> a skos:Concept;
skos:prefLabel "Massif"@en .
<http://resource.geolba.ac.at/geoconnect3d/36> skos:narrower <http://resource.geolba.ac.at/geoconnect3d/40> .
<http://resource.geolba.ac.at/geoconnect3d/40> skos:broader <http://resource.geolba.ac.at/geoconnect3d/36>;
dcterms:created "2020-02-18T12:14:38.856Z"^^xsd:dateTime;
skos:notation "U2_05";
skos:definition "Topographic and/or structural feature commonly formed of rocks more rigid than the surroundings (Neuendorf et al., 2005)."@en .
<http://resource.geolba.ac.at/geoconnect3d/41> a skos:Concept;
skos:prefLabel "Block"@en .
<http://resource.geolba.ac.at/geoconnect3d/36> skos:narrower <http://resource.geolba.ac.at/geoconnect3d/41> .
<http://resource.geolba.ac.at/geoconnect3d/41> skos:broader <http://resource.geolba.ac.at/geoconnect3d/36>;
dcterms:created "2020-02-18T12:14:38.899Z"^^xsd:dateTime;
skos:notation "U2_06";
skos:definition "Solid mass of rock that has been transported with respect to adjacent rock mases through tectonic processes (Neuendorf et al., 2005)."@en .
<http://resource.geolba.ac.at/geoconnect3d/42> a skos:Concept;
skos:prefLabel "Inlier"@en .
<http://resource.geolba.ac.at/geoconnect3d/36> skos:narrower <http://resource.geolba.ac.at/geoconnect3d/42> .
<http://resource.geolba.ac.at/geoconnect3d/42> skos:broader <http://resource.geolba.ac.at/geoconnect3d/36>;
dcterms:created "2020-02-18T12:14:38.937Z"^^xsd:dateTime;
skos:notation "U2_07";
skos:definition "Area or group of rocks surrounded by younger rocks (Neuendorf et al., 2005)."@en .
<http://resource.geolba.ac.at/geoconnect3d/43> a skos:Concept;
skos:prefLabel "Orogenic zone"@en .
<http://resource.geolba.ac.at/geoconnect3d/36> skos:narrower <http://resource.geolba.ac.at/geoconnect3d/43> .
<http://resource.geolba.ac.at/geoconnect3d/43> skos:broader <http://resource.geolba.ac.at/geoconnect3d/36>;
dcterms:created "2020-02-18T12:14:39.092Z"^^xsd:dateTime;
skos:notation "U2_08";
skos:definition "Fault-bounded region that has been subjected to folding and other deformation within an orogen."@en .
<http://resource.geolba.ac.at/geoconnect3d/44> a skos:Concept;
skos:prefLabel "Nappe system"@en .
<http://resource.geolba.ac.at/geoconnect3d/36> skos:narrower <http://resource.geolba.ac.at/geoconnect3d/44> .
<http://resource.geolba.ac.at/geoconnect3d/44> skos:broader <http://resource.geolba.ac.at/geoconnect3d/36>;
dcterms:created "2020-02-18T12:14:39.249Z"^^xsd:dateTime;
skos:notation "U2_09";
skos:definition "Several nappes which originate from neighbouring paleogeographic realms that share a common tectonic history over a certain geological time period. Nappe systems are bound in spatial extent by discrete fault zones similar to nappes (GBA Thesaurus)."@en .
<http://resource.geolba.ac.at/geoconnect3d/45> a skos:Concept;
skos:prefLabel "Nappe"@en .
<http://resource.geolba.ac.at/geoconnect3d/44> skos:narrower <http://resource.geolba.ac.at/geoconnect3d/45> .
<http://resource.geolba.ac.at/geoconnect3d/45> skos:broader <http://resource.geolba.ac.at/geoconnect3d/44>;
dcterms:created "2020-02-18T12:14:39.349Z"^^xsd:dateTime;
skos:notation "U2_10";
skos:definition "Allochthonous sheet-like rock unit that moved on a predominantly horizontal surface to the top of other surfaces (Neuendorf et al. 2005; GBA Thesaurus)."@en .
<http://resource.geolba.ac.at/geoconnect3d/46> a skos:Concept;
skos:prefLabel "Craton"@en .
<http://resource.geolba.ac.at/geoconnect3d/36> skos:narrower <http://resource.geolba.ac.at/geoconnect3d/46> .
<http://resource.geolba.ac.at/geoconnect3d/46> skos:broader <http://resource.geolba.ac.at/geoconnect3d/36>;
dcterms:created "2020-02-18T12:14:39.399Z"^^xsd:dateTime;
skos:notation "U2_11";
skos:definition "Stable part of the crust that has been little deformed for a prolonged period (Neuendorf et al. 2005)."@en .
<http://resource.geolba.ac.at/geoconnect3d/47> a skos:Concept;
skos:prefLabel "Limit level 1"@en .
<http://resource.geolba.ac.at/geoconnect3d/27> skos:hasTopConcept <http://resource.geolba.ac.at/geoconnect3d/47> .
<http://resource.geolba.ac.at/geoconnect3d/47> skos:topConceptOf <http://resource.geolba.ac.at/geoconnect3d/27>;
dcterms:created "2020-02-18T12:14:39.483Z"^^xsd:dateTime .
<http://resource.geolba.ac.at/geoconnect3d/84> a skos:Concept;
skos:prefLabel "Neuendorf et al (2005)"@en;
dcterms:created "2020-02-18T12:26:47.258Z"^^xsd:dateTime;
dcterms:bibliographicCitation "Neuendorf, K.K.E., Mehl, J.P.E. Jr., Jackson, J.E. (2005): Glossary of geology. – 779 S., Alexandria, Virginia (Springer Science & Business Media)." .
<http://resource.geolba.ac.at/geoconnect3d/85> a skos:Concept;
skos:prefLabel "Kearey P., Vine F.J. (1995)"@en;
dcterms:created "2020-02-18T12:26:47.289Z"^^xsd:dateTime;
dcterms:bibliographicCitation "Kearey, P., Vine, F.J. (1995): Global tectonics. Blackwell Science, Oxford, 302 p." .
<http://resource.geolba.ac.at/geoconnect3d/86> a skos:Concept;
skos:prefLabel "GBA (2019)"@en;
dcterms:created "2020-02-18T12:26:47.325Z"^^xsd:dateTime;
dcterms:bibliographicCitation "GBA - Geological Survey of Austria (2019): Thesaurus. Accessed at http://resource.geolba.ac.at/" .
<http://resource.geolba.ac.at/geoconnect3d/87> a skos:Concept;
skos:prefLabel "Passchier C.W., Trouw R.A. (1996)"@en;
dcterms:created "2020-02-18T12:26:47.360Z"^^xsd:dateTime;
dcterms:bibliographicCitation "Passchier, C.W., Trouw, R.A. (1996): Microtectonics. - 289 S., Berlin (Springer)." .
<http://resource.geolba.ac.at/geoconnect3d/88> a skos:Concept;
skos:prefLabel "Hintersberger et al (2017)"@en;
dcterms:created "2020-02-18T12:26:47.395Z"^^xsd:dateTime;
dcterms:bibliographicCitation "Hintersberger, E., Iglseder, C., Schuster, R., Huet, B. (2017): The new database “Tectonic Boundaries” at the Geological Survey of Austria." .
<http://resource.geolba.ac.at/geoconnect3d/89> a skos:Concept;
skos:prefLabel "GeoConnect³d"@en .
<http://resource.geolba.ac.at/geoconnect3d/23> skos:hasTopConcept <http://resource.geolba.ac.at/geoconnect3d/89> .
<http://resource.geolba.ac.at/geoconnect3d/89> skos:topConceptOf <http://resource.geolba.ac.at/geoconnect3d/23>;
dcterms:created "2020-02-18T12:26:47.445Z"^^xsd:dateTime .
<http://resource.geolba.ac.at/geoconnect3d/90> a skos:Concept;
skos:prefLabel "Geluk et al (1994)"@en;
dcterms:created "2020-02-18T12:26:47.478Z"^^xsd:dateTime;
dcterms:bibliographicCitation "Geluk M.C. et al. (1994): Stratigraphy and tectonics of the Roer Valley Graben. Geologie en Mijnbouw 73, 129-141" .
<http://resource.geolba.ac.at/geoconnect3d/91> a skos:Concept;
skos:prefLabel "Ziegler (1990)"@en;
dcterms:created "2020-02-18T12:26:47.510Z"^^xsd:dateTime;
dcterms:bibliographicCitation "Ziegler P.A. (1990): Geological atlas of western and central Europe. Shell/Elsevier Sci Publ, 155 pp" .
<http://resource.geolba.ac.at/geoconnect3d/48> skos:broader <http://resource.geolba.ac.at/geoconnect3d/47>;
dcterms:created "2020-02-18T12:14:39.526Z"^^xsd:dateTime;
skos:notation "L1_02";
skos:definition "Alignment of connected and kinematically related fault systems with extension of hundreds of km and transregional impact in the geological evolution (Hintersberger et al., 2017)."@en;
skos:example "Roer Valley Graben large-scale fault system"@en .
<http://resource.geolba.ac.at/geoconnect3d/49> a skos:Concept;
skos:prefLabel "Fault system"@en .
<http://resource.geolba.ac.at/geoconnect3d/48> skos:narrower <http://resource.geolba.ac.at/geoconnect3d/49> .
<http://resource.geolba.ac.at/geoconnect3d/49> skos:broader <http://resource.geolba.ac.at/geoconnect3d/48>;
dcterms:created "2020-02-18T12:14:39.669Z"^^xsd:dateTime;
skos:notation "L1_03";
skos:definition "Alignment of connected and kinematically related faults and/or shear zones active during at least one or potentially several geological events, may contain different deformation styles (Hintersberger et al., 2017)."@en;
skos:example "Peel Boundary fault zone"@en .
<http://resource.geolba.ac.at/geoconnect3d/50> a skos:Concept;
skos:prefLabel "Fault"@en .
<http://resource.geolba.ac.at/geoconnect3d/49> skos:narrower <http://resource.geolba.ac.at/geoconnect3d/50> .
<http://resource.geolba.ac.at/geoconnect3d/50> skos:broader <http://resource.geolba.ac.at/geoconnect3d/49>;
dcterms:created "2020-02-18T12:14:39.744Z"^^xsd:dateTime;
skos:notation "L1_04";
skos:definition "Discrete deforming interface separating two rock masses along which one mass has slid past the other (Neuendorf et al., 2005)."@en;
skos:example "Rauw fault"@en .
<http://resource.geolba.ac.at/geoconnect3d/51> a skos:Concept;
skos:prefLabel "Subfault"@en .
<http://resource.geolba.ac.at/geoconnect3d/50> skos:narrower <http://resource.geolba.ac.at/geoconnect3d/51> .
<http://resource.geolba.ac.at/geoconnect3d/51> skos:broader <http://resource.geolba.ac.at/geoconnect3d/50>;
dcterms:created "2020-02-18T12:14:39.800Z"^^xsd:dateTime;
skos:notation "L1_05";
skos:definition "Subordinated discrete interface separating two rock masses along which one mass has slid past the other, belonging to an ordinated fault (Neuendorf et al. 2005; Hintersberger et al., 2017)."@en;
skos:example "Rauw 1 fault"@en .
<http://resource.geolba.ac.at/geoconnect3d/52> a skos:Concept;
skos:prefLabel "Fault set"@en .
<http://resource.geolba.ac.at/geoconnect3d/47> skos:narrower <http://resource.geolba.ac.at/geoconnect3d/52> .
<http://resource.geolba.ac.at/geoconnect3d/52> skos:broader <http://resource.geolba.ac.at/geoconnect3d/47>;
dcterms:created "2020-02-18T12:14:39.835Z"^^xsd:dateTime;
skos:notation "L1_06";
skos:definition "Alignment of parallel trending faults that are kinematically and temporarily linked, but spacing between faults exceeds the displacement along the fault (Hintersberger et al., 2017)."@en .
<http://resource.geolba.ac.at/geoconnect3d/53> a skos:Concept;
skos:prefLabel "Deformation front"@en .
<http://resource.geolba.ac.at/geoconnect3d/47> skos:narrower <http://resource.geolba.ac.at/geoconnect3d/53> .
<http://resource.geolba.ac.at/geoconnect3d/53> skos:broader <http://resource.geolba.ac.at/geoconnect3d/47>;
dcterms:created "2020-02-18T12:14:39.924Z"^^xsd:dateTime;
skos:notation "L1_07";
skos:definition "Outermost zone of an orogen."@en;
skos:example "Variscan front zone"@en .
<http://resource.geolba.ac.at/geoconnect3d/54> a skos:Concept;
skos:prefLabel "Plate boundary"@en .
<http://resource.geolba.ac.at/geoconnect3d/47> skos:narrower <http://resource.geolba.ac.at/geoconnect3d/54> .
<http://resource.geolba.ac.at/geoconnect3d/54> skos:broader <http://resource.geolba.ac.at/geoconnect3d/47>;
dcterms:created "2020-02-18T12:14:39.989Z"^^xsd:dateTime .
<http://resource.geolba.ac.at/geoconnect3d/86> a dcterms:BibliographicResource .
<http://resource.geolba.ac.at/geoconnect3d/90> a dcterms:BibliographicResource .
<http://resource.geolba.ac.at/geoconnect3d/89> a dcterms:BibliographicResource .
<http://resource.geolba.ac.at/geoconnect3d/87> a dcterms:BibliographicResource .
<http://resource.geolba.ac.at/geoconnect3d/88> a dcterms:BibliographicResource .
<http://resource.geolba.ac.at/geoconnect3d/85> a dcterms:BibliographicResource .
<http://resource.geolba.ac.at/geoconnect3d/91> a dcterms:BibliographicResource .
<http://resource.geolba.ac.at/geoconnect3d/84> a dcterms:BibliographicResource .
<http://resource.geolba.ac.at/geoconnect3d/20> dcterms:modified "2020-02-07T14:55:42.971Z"^^xsd:dateTime .
<http://resource.geolba.ac.at/geoconnect3d/22> dcterms:modified "2020-02-07T14:56:16.752Z"^^xsd:dateTime .
<http://resource.geolba.ac.at/geoconnect3d/21> dcterms:modified "2020-02-07T14:56:29.099Z"^^xsd:dateTime .
<http://resource.geolba.ac.at/geoconnect3d/6> dcterms:modified "2020-02-07T14:58:15.379Z"^^xsd:dateTime .
<http://resource.geolba.ac.at/geoconnect3d/5> dcterms:modified "2020-02-07T14:57:54.987Z"^^xsd:dateTime .
<http://resource.geolba.ac.at/geoconnect3d/11> dcterms:modified "2020-02-07T14:58:53.535Z"^^xsd:dateTime .
<http://resource.geolba.ac.at/geoconnect3d/10> dcterms:modified "2020-02-07T14:59:04.495Z"^^xsd:dateTime .
<http://resource.geolba.ac.at/geoconnect3d/2> dcterms:modified "2020-02-07T14:57:45.115Z"^^xsd:dateTime .
<http://resource.geolba.ac.at/geoconnect3d/9> dcterms:modified "2020-02-07T14:57:20.589Z"^^xsd:dateTime .
<http://resource.geolba.ac.at/geoconnect3d/8> dcterms:modified "2020-02-07T14:58:43.257Z"^^xsd:dateTime .
<http://resource.geolba.ac.at/geoconnect3d/7> dcterms:modified "2020-02-07T14:58:35.033Z"^^xsd:dateTime .
<http://resource.geolba.ac.at/geoconnect3d/17> dcterms:modified "2020-02-07T14:55:28.075Z"^^xsd:dateTime .
<http://resource.geolba.ac.at/geoconnect3d/16> dcterms:modified "2020-02-07T14:55:03.814Z"^^xsd:dateTime .
<http://resource.geolba.ac.at/geoconnect3d/19> dcterms:modified "2020-02-07T14:56:01.601Z"^^xsd:dateTime .
<http://resource.geolba.ac.at/geoconnect3d/18> dcterms:modified "2020-02-07T14:55:53.305Z"^^xsd:dateTime .
<http://resource.geolba.ac.at/geoconnect3d/13> dcterms:modified "2020-02-07T14:54:11.722Z"^^xsd:dateTime .
<http://resource.geolba.ac.at/geoconnect3d/15> a <http://resource.geolba.ac.at/schema/GeoConnect#limit>;
dcterms:modified "2020-02-07T14:55:15.140Z"^^xsd:dateTime .
<http://resource.geolba.ac.at/geoconnect3d/14> dcterms:modified "2020-02-07T14:54:52.830Z"^^xsd:dateTime .
<http://resource.geolba.ac.at/geoconnect3d/47> dcterms:modified "2020-02-18T12:37:14.140Z"^^xsd:dateTime;
dcterms:references <http://resource.geolba.ac.at/geoconnect3d/89> .
<http://resource.geolba.ac.at/geoconnect3d/55> dcterms:references <http://resource.geolba.ac.at/geoconnect3d/89>;
dcterms:modified "2020-02-18T12:37:29.002Z"^^xsd:dateTime .
<http://resource.geolba.ac.at/geoconnect3d/53> dcterms:references <http://resource.geolba.ac.at/geoconnect3d/89>;
dcterms:modified "2020-02-18T12:37:40.888Z"^^xsd:dateTime .
<http://resource.geolba.ac.at/geoconnect3d/52> dcterms:modified "2020-02-18T12:37:50.687Z"^^xsd:dateTime;
dcterms:references <http://resource.geolba.ac.at/geoconnect3d/88> .
<http://resource.geolba.ac.at/geoconnect3d/48> dcterms:modified "2020-02-18T14:44:57.462Z"^^xsd:dateTime;
dcterms:references <http://resource.geolba.ac.at/geoconnect3d/88> .
<http://resource.geolba.ac.at/geoconnect3d/49> dcterms:references <http://resource.geolba.ac.at/geoconnect3d/88> .
<http://resource.geolba.ac.at/geoconnect3d/50> dcterms:references <http://resource.geolba.ac.at/geoconnect3d/88> .
<http://resource.geolba.ac.at/geoconnect3d/51> dcterms:references <http://resource.geolba.ac.at/geoconnect3d/88> .
<http://resource.geolba.ac.at/geoconnect3d/54> dcterms:modified "2020-02-18T12:39:02.907Z"^^xsd:dateTime;
dcterms:references <http://resource.geolba.ac.at/geoconnect3d/85> .
<http://resource.geolba.ac.at/geoconnect3d/51> dcterms:references <http://resource.geolba.ac.at/geoconnect3d/84> .
<http://resource.geolba.ac.at/geoconnect3d/56> dcterms:references <http://resource.geolba.ac.at/geoconnect3d/89>;
dcterms:modified "2020-02-18T12:40:05.608Z"^^xsd:dateTime .
<http://resource.geolba.ac.at/geoconnect3d/57> dcterms:references <http://resource.geolba.ac.at/geoconnect3d/87>;
dcterms:modified "2020-02-18T12:40:25.743Z"^^xsd:dateTime .
<http://resource.geolba.ac.at/geoconnect3d/72> dcterms:modified "2020-02-18T12:41:10.332Z"^^xsd:dateTime;
dcterms:references <http://resource.geolba.ac.at/geoconnect3d/85> .
<http://resource.geolba.ac.at/geoconnect3d/73> dcterms:modified "2020-02-18T12:41:25.779Z"^^xsd:dateTime;
dcterms:references <http://resource.geolba.ac.at/geoconnect3d/84> .
<http://resource.geolba.ac.at/geoconnect3d/74> dcterms:modified "2020-02-18T12:41:40.702Z"^^xsd:dateTime;
dcterms:references <http://resource.geolba.ac.at/geoconnect3d/84> .
<http://resource.geolba.ac.at/geoconnect3d/75> dcterms:references <http://resource.geolba.ac.at/geoconnect3d/89>;
dcterms:modified "2020-02-18T12:41:59.402Z"^^xsd:dateTime .
<http://resource.geolba.ac.at/geoconnect3d/28> dcterms:modified "2020-02-18T12:42:51.079Z"^^xsd:dateTime;
dcterms:references <http://resource.geolba.ac.at/geoconnect3d/84> .
<http://resource.geolba.ac.at/geoconnect3d/29> dcterms:modified "2020-02-18T12:43:02.505Z"^^xsd:dateTime;
dcterms:references <http://resource.geolba.ac.at/geoconnect3d/84> .
<http://resource.geolba.ac.at/geoconnect3d/30> dcterms:modified "2020-02-18T12:43:13.686Z"^^xsd:dateTime;
dcterms:references <http://resource.geolba.ac.at/geoconnect3d/84> .
<http://resource.geolba.ac.at/geoconnect3d/31> dcterms:references <http://resource.geolba.ac.at/geoconnect3d/86>;
dcterms:modified "2020-02-18T12:43:25.532Z"^^xsd:dateTime .
<http://resource.geolba.ac.at/geoconnect3d/32> dcterms:references <http://resource.geolba.ac.at/geoconnect3d/84>;
dcterms:modified "2020-02-18T12:43:34.916Z"^^xsd:dateTime .
<http://resource.geolba.ac.at/geoconnect3d/34> dcterms:references <http://resource.geolba.ac.at/geoconnect3d/84> .
<http://resource.geolba.ac.at/geoconnect3d/35> dcterms:modified "2020-02-18T12:44:14.073Z"^^xsd:dateTime;
dcterms:references <http://resource.geolba.ac.at/geoconnect3d/85> .
<http://resource.geolba.ac.at/geoconnect3d/34> dcterms:references <http://resource.geolba.ac.at/geoconnect3d/86>;
skos:example "Variscan orogen"@en;
dcterms:modified "2020-02-18T12:44:52.346Z"^^xsd:dateTime .
<http://resource.geolba.ac.at/geoconnect3d/36> dcterms:modified "2020-02-18T12:45:46.820Z"^^xsd:dateTime;
dcterms:references <http://resource.geolba.ac.at/geoconnect3d/89> .
<http://resource.geolba.ac.at/geoconnect3d/41> dcterms:modified "2020-02-18T12:45:56.475Z"^^xsd:dateTime;
dcterms:references <http://resource.geolba.ac.at/geoconnect3d/84> .
<http://resource.geolba.ac.at/geoconnect3d/46> dcterms:references <http://resource.geolba.ac.at/geoconnect3d/84>;
dcterms:modified "2020-02-18T12:46:06.483Z"^^xsd:dateTime .
<http://resource.geolba.ac.at/geoconnect3d/37> dcterms:modified "2020-02-18T12:46:16.531Z"^^xsd:dateTime;
dcterms:references <http://resource.geolba.ac.at/geoconnect3d/84> .
<http://resource.geolba.ac.at/geoconnect3d/38> dcterms:modified "2020-02-18T12:46:24.341Z"^^xsd:dateTime;
dcterms:references <http://resource.geolba.ac.at/geoconnect3d/84> .
<http://resource.geolba.ac.at/geoconnect3d/42> dcterms:references <http://resource.geolba.ac.at/geoconnect3d/84>;
dcterms:modified "2020-02-18T12:46:34.058Z"^^xsd:dateTime .
<http://resource.geolba.ac.at/geoconnect3d/40> dcterms:references <http://resource.geolba.ac.at/geoconnect3d/84>;
dcterms:modified "2020-02-18T12:46:42.104Z"^^xsd:dateTime .
<http://resource.geolba.ac.at/geoconnect3d/44> dcterms:references <http://resource.geolba.ac.at/geoconnect3d/86> .
<http://resource.geolba.ac.at/geoconnect3d/45> dcterms:references <http://resource.geolba.ac.at/geoconnect3d/84> .
<http://resource.geolba.ac.at/geoconnect3d/43> dcterms:modified "2020-02-18T12:47:09.448Z"^^xsd:dateTime;
dcterms:references <http://resource.geolba.ac.at/geoconnect3d/84> .
<http://resource.geolba.ac.at/geoconnect3d/45> dcterms:references <http://resource.geolba.ac.at/geoconnect3d/86> .
<http://resource.geolba.ac.at/geoconnect3d/26> skos:broader <http://resource.geolba.ac.at/geoconnect3d/89> .
<http://resource.geolba.ac.at/geoconnect3d/89> skos:narrower <http://resource.geolba.ac.at/geoconnect3d/26> .
<http://resource.geolba.ac.at/geoconnect3d/25> skos:broader <http://resource.geolba.ac.at/geoconnect3d/89> .
<http://resource.geolba.ac.at/geoconnect3d/89> skos:narrower <http://resource.geolba.ac.at/geoconnect3d/25>,<http://resource.geolba.ac.at/geoconnect3d/86> .
<http://resource.geolba.ac.at/geoconnect3d/86> skos:broader <http://resource.geolba.ac.at/geoconnect3d/89> .
<http://resource.geolba.ac.at/geoconnect3d/90> skos:broader <http://resource.geolba.ac.at/geoconnect3d/89> .
<http://resource.geolba.ac.at/geoconnect3d/89> skos:narrower <http://resource.geolba.ac.at/geoconnect3d/90> .
<http://resource.geolba.ac.at/geoconnect3d/88> skos:broader <http://resource.geolba.ac.at/geoconnect3d/89> .
<http://resource.geolba.ac.at/geoconnect3d/89> skos:narrower <http://resource.geolba.ac.at/geoconnect3d/88>,<http://resource.geolba.ac.at/geoconnect3d/85> .
<http://resource.geolba.ac.at/geoconnect3d/85> skos:broader <http://resource.geolba.ac.at/geoconnect3d/89> .
<http://resource.geolba.ac.at/geoconnect3d/26> dcterms:modified "2020-02-18T12:56:31.046Z"^^xsd:dateTime .
<http://resource.geolba.ac.at/geoconnect3d/25> dcterms:modified "2020-02-18T12:56:31.822Z"^^xsd:dateTime .
<http://resource.geolba.ac.at/geoconnect3d/86> dcterms:modified "2020-02-18T12:56:32.646Z"^^xsd:dateTime .
<http://resource.geolba.ac.at/geoconnect3d/88> dcterms:modified "2020-02-18T12:56:35.749Z"^^xsd:dateTime .
<http://resource.geolba.ac.at/geoconnect3d/85> dcterms:modified "2020-02-18T12:56:36.902Z"^^xsd:dateTime .
<http://resource.geolba.ac.at/geoconnect3d/89> skos:narrower <http://resource.geolba.ac.at/geoconnect3d/84> .
<http://resource.geolba.ac.at/geoconnect3d/84> skos:broader <http://resource.geolba.ac.at/geoconnect3d/89> .
<http://resource.geolba.ac.at/geoconnect3d/89> skos:narrower <http://resource.geolba.ac.at/geoconnect3d/87> .
<http://resource.geolba.ac.at/geoconnect3d/87> skos:broader <http://resource.geolba.ac.at/geoconnect3d/89>;
dcterms:modified "2020-02-18T12:57:21.106Z"^^xsd:dateTime .
<http://resource.geolba.ac.at/geoconnect3d/89> skos:narrower <http://resource.geolba.ac.at/geoconnect3d/91> .
<http://resource.geolba.ac.at/geoconnect3d/91> skos:broader <http://resource.geolba.ac.at/geoconnect3d/89> .
<http://resource.geolba.ac.at/geoconnect3d/84> dcterms:modified "2020-02-18T12:57:20.298Z"^^xsd:dateTime .
<http://resource.geolba.ac.at/geoconnect3d/1> skos:altLabel "Roer Valley graben large-scale fault system"@en;
skos:scopeNote "Mesozoic, Cenozoic"@en .
<http://resource.geolba.ac.at/geoconnect3d/92> a skos:Concept;
dcterms:created "2020-02-18T13:01:20.286Z"^^xsd:dateTime .
<http://resource.geolba.ac.at/geoconnect3d/0> skos:hasTopConcept <http://resource.geolba.ac.at/geoconnect3d/92> .
<http://resource.geolba.ac.at/geoconnect3d/92> skos:prefLabel "Roer Valley graben"@en;
skos:topConceptOf <http://resource.geolba.ac.at/geoconnect3d/0>;
a <http://resource.geolba.ac.at/schema/GeoConnect#unit> .
<http://resource.geolba.ac.at/geoconnect3d/1> skos:notation "GSB_001";
skos:scopeNote "(we would like to use scopeNote to include a few lines on the interpretation)"@en,"Group of faults limiting the Roer Valley graben."@en;
a <http://resource.geolba.ac.at/schema/GeoConnect#limit> .
<http://resource.geolba.ac.at/geoconnect3d/12> dcterms:modified "2020-02-18T13:44:40.567Z"^^xsd:dateTime .
<http://resource.geolba.ac.at/geoconnect3d/19> a <http://resource.geolba.ac.at/schema/GeoConnect#limit> .
<http://resource.geolba.ac.at/geoconnect3d/12> a <http://resource.geolba.ac.at/schema/GeoConnect#limit> .
<http://resource.geolba.ac.at/geoconnect3d/17> a <http://resource.geolba.ac.at/schema/GeoConnect#limit> .
<http://resource.geolba.ac.at/geoconnect3d/18> a <http://resource.geolba.ac.at/schema/GeoConnect#limit> .
<http://resource.geolba.ac.at/geoconnect3d/16> a <http://resource.geolba.ac.at/schema/GeoConnect#limit> .
<http://resource.geolba.ac.at/geoconnect3d/20> a <http://resource.geolba.ac.at/schema/GeoConnect#limit> .
<http://resource.geolba.ac.at/geoconnect3d/13> a <http://resource.geolba.ac.at/schema/GeoConnect#limit> .
<http://resource.geolba.ac.at/geoconnect3d/14> a <http://resource.geolba.ac.at/schema/GeoConnect#limit> .
<http://resource.geolba.ac.at/geoconnect3d/21> a <http://resource.geolba.ac.at/schema/GeoConnect#limit> .
<http://resource.geolba.ac.at/geoconnect3d/22> a <http://resource.geolba.ac.at/schema/GeoConnect#limit> .
<http://resource.geolba.ac.at/geoconnect3d/7> a <http://resource.geolba.ac.at/schema/GeoConnect#limit> .
<http://resource.geolba.ac.at/geoconnect3d/10> a <http://resource.geolba.ac.at/schema/GeoConnect#limit> .
<http://resource.geolba.ac.at/geoconnect3d/6> a <http://resource.geolba.ac.at/schema/GeoConnect#limit> .
<http://resource.geolba.ac.at/geoconnect3d/8> a <http://resource.geolba.ac.at/schema/GeoConnect#limit> .
<http://resource.geolba.ac.at/geoconnect3d/9> a <http://resource.geolba.ac.at/schema/GeoConnect#limit> .
<http://resource.geolba.ac.at/geoconnect3d/4> a <http://resource.geolba.ac.at/schema/GeoConnect#limit> .
<http://resource.geolba.ac.at/geoconnect3d/11> a <http://resource.geolba.ac.at/schema/GeoConnect#limit> .
<http://resource.geolba.ac.at/geoconnect3d/5> a <http://resource.geolba.ac.at/schema/GeoConnect#limit> .
<http://resource.geolba.ac.at/geoconnect3d/2> a <http://resource.geolba.ac.at/schema/GeoConnect#limit> .
<http://resource.geolba.ac.at/geoconnect3d/3> a <http://resource.geolba.ac.at/schema/GeoConnect#limit> .
<http://resource.geolba.ac.at/geoconnect3d/92> skos:definition "Asymmetric Cenozoic graben filled with up to 2000m of predominantly Upper Oligocene to Quaternary sediments (Geluk et al., 1994)."@en;
skos:scopeNote "The Roer Valley graben forms the northwestern branch of the Rhine Graben rift system (Ziegler, 1990)"@en;
dcterms:references <http://resource.geolba.ac.at/geoconnect3d/90> .
<http://resource.geolba.ac.at/geoconnect3d/90> dcterms:modified "2020-02-18T13:50:18.036Z"^^xsd:dateTime .
<http://resource.geolba.ac.at/geoconnect3d/92> dcterms:references <http://resource.geolba.ac.at/geoconnect3d/91> .
<http://resource.geolba.ac.at/geoconnect3d/91> dcterms:modified "2020-02-18T13:50:23.588Z"^^xsd:dateTime .
<http://resource.geolba.ac.at/geoconnect3d/23> dcterms:modified "2020-02-19T13:08:19.309Z"^^xsd:dateTime .
<http://resource.geolba.ac.at/geoconnect3d/27> dcterms:modified "2020-02-19T13:09:12.598Z"^^xsd:dateTime .
<http://resource.geolba.ac.at/geoconnect3d/48> skos:exactMatch <http://resource.geolba.ac.at/structure/64> .
<http://resource.geolba.ac.at/geoconnect3d/49> skos:exactMatch <http://resource.geolba.ac.at/structure/65>;
dcterms:modified "2020-02-18T14:45:15.490Z"^^xsd:dateTime .
<http://resource.geolba.ac.at/geoconnect3d/50> skos:exactMatch <http://resource.geolba.ac.at/structure/28>;
dcterms:modified "2020-02-18T14:45:32.770Z"^^xsd:dateTime .
<http://resource.geolba.ac.at/geoconnect3d/51> skos:exactMatch <http://resource.geolba.ac.at/structure/67>;
dcterms:modified "2020-02-18T14:45:50.968Z"^^xsd:dateTime .
<http://resource.geolba.ac.at/geoconnect3d/45> skos:exactMatch <http://resource.geolba.ac.at/tectonicunit/15>;
dcterms:modified "2020-02-18T14:47:05.516Z"^^xsd:dateTime .
<http://resource.geolba.ac.at/geoconnect3d/44> skos:exactMatch <http://resource.geolba.ac.at/tectonicunit/14>;
dcterms:modified "2020-02-18T14:47:18.787Z"^^xsd:dateTime .
<http://resource.geolba.ac.at/geoconnect3d/92> skos:notation "VITO_10001" .
<http://resource.geolba.ac.at/geoconnect3d/1> dcterms:modified "2020-02-18T14:55:10.582Z"^^xsd:dateTime .
<http://resource.geolba.ac.at/geoconnect3d/3> <http://resource.geolba.ac.at/schema/GeoConnect#limitTo> <http://resource.geolba.ac.at/geoconnect3d/92> .
<http://resource.geolba.ac.at/geoconnect3d/92> <http://resource.geolba.ac.at/schema/GeoConnect#limitedBy> <http://resource.geolba.ac.at/geoconnect3d/3> .
<http://resource.geolba.ac.at/geoconnect3d/3> dcterms:modified "2020-02-18T14:55:23.909Z"^^xsd:dateTime .
<http://resource.geolba.ac.at/geoconnect3d/4> <http://resource.geolba.ac.at/schema/GeoConnect#limitTo> <http://resource.geolba.ac.at/geoconnect3d/92> .
<http://resource.geolba.ac.at/geoconnect3d/92> <http://resource.geolba.ac.at/schema/GeoConnect#limitedBy> <http://resource.geolba.ac.at/geoconnect3d/4> .
<http://resource.geolba.ac.at/geoconnect3d/4> dcterms:modified "2020-02-18T14:55:31.524Z"^^xsd:dateTime .
<http://resource.geolba.ac.at/geoconnect3d/92> skos:exactMatch <http://www.wikidata.org/entity/Q2251458>;
foaf:page <https://nl.wikipedia.org/wiki/Roerdalslenk>;
foaf:depiction <https://i2.wp.com/geoera.eu/wp-content/uploads/2019/10/VITO_Fig1.jpg>;
<https://schema.org/mainEntityOfPage> <https://www.youtube.com/watch?v=YjRywrshzu0>;
dcterms:modified "2020-02-20T10:57:11.313Z"^^xsd:dateTime .
<http://resource.geolba.ac.at/geoconnect3d/89> dcterms:modified "2020-02-19T13:04:29.818Z"^^xsd:dateTime .
<http://resource.geolba.ac.at/geoconnect3d/27> dcterms:description ".. here a description of the concept schema .."@en .
<http://resource.geolba.ac.at/geoconnect3d/0> dcterms:description ".. here a description of the concept schema .."@en .
<http://resource.geolba.ac.at/geoconnect3d/23> dcterms:description ".. here a description of selected bibliographic references .."@en;
dcterms:title "References"@en .
<http://resource.geolba.ac.at/geoconnect3d/0> dcterms:title "Geologic features"@en;
dcterms:modified "2020-02-19T13:08:40.594Z"^^xsd:dateTime .
<http://resource.geolba.ac.at/geoconnect3d/27> dcterms:title "Classification of units and limits"@en .
<http://resource.geolba.ac.at/geoconnect3d/62> skos:exactMatch <http://inspire.ec.europa.eu/codelist/FaultTypeValue/detachmentFault>;
dcterms:modified "2020-02-19T14:47:35.976Z"^^xsd:dateTime .
<http://resource.geolba.ac.at/geoconnect3d/64> skos:exactMatch <http://inspire.ec.europa.eu/codelist/FaultTypeValue/extractionFault>;
dcterms:modified "2020-02-19T14:47:49.254Z"^^xsd:dateTime .
<http://resource.geolba.ac.at/geoconnect3d/63> dcterms:modified "2020-02-19T14:48:03.502Z"^^xsd:dateTime;
skos:exactMatch <http://inspire.ec.europa.eu/codelist/FaultTypeValue/horizontalFault> .
<http://resource.geolba.ac.at/geoconnect3d/58> dcterms:modified "2020-02-19T14:48:21.532Z"^^xsd:dateTime;
skos:exactMatch <http://inspire.ec.europa.eu/codelist/FaultTypeValue/normalFault> .
<http://resource.geolba.ac.at/geoconnect3d/67> dcterms:modified "2020-02-19T14:48:38.051Z"^^xsd:dateTime;
skos:exactMatch <http://inspire.ec.europa.eu/codelist/FaultTypeValue/obliqueSlipFault> .
<http://resource.geolba.ac.at/geoconnect3d/59> dcterms:modified "2020-02-19T14:48:51.905Z"^^xsd:dateTime;
skos:exactMatch <http://inspire.ec.europa.eu/codelist/FaultTypeValue/reverseFault> .
<http://resource.geolba.ac.at/geoconnect3d/68> dcterms:modified "2020-02-19T14:49:04.634Z"^^xsd:dateTime;
skos:exactMatch <http://inspire.ec.europa.eu/codelist/FaultTypeValue/scissorFault> .
<http://resource.geolba.ac.at/geoconnect3d/60> skos:exactMatch <http://inspire.ec.europa.eu/codelist/FaultTypeValue/strikeSlipFault>;
dcterms:modified "2020-02-19T14:49:27.136Z"^^xsd:dateTime .
<http://resource.geolba.ac.at/geoconnect3d/61> skos:exactMatch <http://inspire.ec.europa.eu/codelist/FaultTypeValue/thrustFault>;
dcterms:modified "2020-02-19T14:49:47.008Z"^^xsd:dateTime .
<http://resource.geolba.ac.at/geoconnect3d/69> dcterms:modified "2020-02-19T14:50:02.406Z"^^xsd:dateTime;
skos:exactMatch <http://inspire.ec.europa.eu/codelist/FaultTypeValue/wrenchFault> .
<http://resource.geolba.ac.at/geoconnect3d/92> skos:exactMatch <http://nl.dbpedia.org/resource/Roerdalslenk>;
skos:altLabel "Roerdalslenk"@nl,"Roerslenk"@nl;
skos:prefLabel "Rurgraben"@de .
}
